prove rev

clightdm/mem/ClightDmMem1.v
@@ -101,59 +101,41 @@ Section PROP.
     else 8
   .
 
-  (* Definition captured_to vaddr m i : iProp := *)
-  (*   match vaddr with *)
-  (*   | Vptr b ofs => *)
-  (*     OwnM (_has_size m.(blk) m.(sz)) *)
-  (*     ** ∃ a, OwnM (_has_base m.(blk) a) *)
-  (*     ** ⌜b = m.(blk) /\ ofs = Ptrofs.sub i a *)
-  (*        /\ Ptrofs.unsigned a + m.(sz) ≤ Ptrofs.max_unsigned⌝ *)
-  (*   | Vint i' => if Archi.ptr64 then False *)
-  (*                else ⌜i = Ptrofs.of_int i'⌝ *)
-  (*   | Vlong i' => if Archi.ptr64 then ⌜i = Ptrofs.of_int64 i'⌝  *)
-  (*                 else False *)
-  (*   | _ => ⌜False⌝ *)
-  (*   end%I. *)
-
   Definition _has_offset vaddr m ofs : iProp :=
     OwnM (_has_size m.(blk) m.(sz))
     ** match vaddr with
        | Vptr b ofs' => ⌜Some b = m.(blk) /\ ofs = ofs'⌝
        | Vint i =>
           if Archi.ptr64 then ⌜False⌝
-          else ∃ a, OwnM (_has_base m.(blk) a) ** ⌜ofs = Ptrofs.sub (Ptrofs.of_int i) a⌝
+          else ∃ a, OwnM (_has_base m.(blk) a) ** ⌜ofs = Ptrofs.sub (Ptrofs.of_int i) a /\ Ptrofs.unsigned a + m.(sz) ≤ Ptrofs.max_unsigned⌝
        | Vlong i =>
           if negb Archi.ptr64 then ⌜False⌝
-          else ∃ a, OwnM (_has_base m.(blk) a) ** ⌜ofs = Ptrofs.sub (Ptrofs.of_int64 i) a⌝
+          else ∃ a, OwnM (_has_base m.(blk) a) ** ⌜ofs = Ptrofs.sub (Ptrofs.of_int64 i) a /\ Ptrofs.unsigned a + m.(sz) ≤ Ptrofs.max_unsigned⌝
        | _ => ⌜False⌝
        end.
 
   Definition equiv_prov vaddr vaddr' m : iProp :=
     ∃ ofs, _has_offset vaddr m ofs ** _has_offset vaddr' m ofs.
 
-  (* Definition metadata_alive m tg q : iProp := *)
-  (*   OwnM (_allocated_with m.(blk) tg q) *)
-  (*   ** OwnM (_has_size m.(blk) m.(sz)). *)
-
   Definition points_to vaddr m mvs q : iProp :=
     match m.(blk) with
     | None => ⌜False⌝
     | Some blk =>
         OwnM (_has_size (Some blk) m.(sz))
-          ** ∃ ofs, OwnM (_points_to blk (Ptrofs.unsigned ofs) mvs q)
-          ** _has_offset vaddr m ofs
-          ** ⌜Ptrofs.unsigned ofs + length mvs ≤ m.(sz)⌝
-          ** match vaddr with
-          | Vptr b ofs'  =>
+        ** ∃ ofs, OwnM (_points_to blk (Ptrofs.unsigned ofs) mvs q)
+        ** _has_offset vaddr m ofs
+        ** ⌜Ptrofs.unsigned ofs + length mvs ≤ m.(sz)⌝
+        ** match vaddr with
+           | Vptr b ofs'  =>
               ⌜Ptrofs.unsigned ofs + length mvs ≤ Ptrofs.max_unsigned⌝
-          | Vint i =>
+           | Vint i =>
               ⌜Ptrofs.unsigned ofs + length mvs ≤ Ptrofs.max_unsigned
               /\ Int.unsigned i + length mvs ≤ Ptrofs.max_unsigned⌝
-          | Vlong i =>
+           | Vlong i =>
               ⌜Ptrofs.unsigned ofs + length mvs ≤ Ptrofs.max_unsigned
               /\ Int64.unsigned i + length mvs ≤ Ptrofs.max_unsigned⌝
-          | _ => ⌜False⌝
-          end
+           | _ => ⌜False⌝
+           end
     end%I.
 
   Definition has_offset vaddr m ofs tg q : iProp :=
@@ -161,6 +143,13 @@ Section PROP.
     | None => ⌜False⌝
     | Some blk => OwnM(_allocated_with blk tg q) ** _has_offset vaddr m ofs
     end%I.
+
+  Definition m_null : metadata.
+  Proof.
+    eapply Build_metadata.
+    instantiate (1:=0).
+    instantiate (1:=None). ss.
+  Qed.
 
   Definition disjoint (m m0: metadata) : Prop :=
     m.(blk) <> m0.(blk).
@@ -173,9 +162,7 @@ Section PROP.
 
 End PROP.
 
-(* Notation "vaddr '(≃_' m ) i " := (captured_to vaddr m i) (at level 10). *)
 Notation "vaddr ⊨ m # ofs" := (_has_offset vaddr m ofs) (at level 10).
-(* Notation "'live_' q # ( m , tg )" := (metadata_alive m tg q) (at level 10). *)
 Notation "vaddr '(↦_' m , q ) mvs" := (points_to vaddr m mvs q) (at level 20).
 Notation "vaddr '(⊨_' m , tg , q ) ofs" := (has_offset vaddr m ofs tg q) (at level 10).
 Notation "m #^ m0" := (disjoint m m0) (at level 20).
@@ -183,11 +170,20 @@ Notation "vaddr '(≃_' m ) vaddr'" := (equiv_prov vaddr vaddr' m) (at level 20)
 
 Section AUX.
 
-  Context `{@GRA.inG pointstoRA Σ}.
-  Context `{@GRA.inG allocatedRA Σ}.
-  Context `{@GRA.inG blocksizeRA Σ}.
-  Context `{@GRA.inG blockaddressRA Σ}.
-
+  Lemma ptrofs_int64_add i k :
+    Archi.ptr64 = true -> Ptrofs.add (Ptrofs.of_int64 i) k = Ptrofs.of_int64 (Int64.add i (Ptrofs.to_int64 k)).
+  Proof.
+    i. unfold Ptrofs.of_int64, Ptrofs.to_int64, Int64.add, Ptrofs.add.
+    rewrite (Int64.unsigned_repr (Ptrofs.unsigned _)).
+    2:{ change Int64.max_unsigned with Ptrofs.max_unsigned.
+        apply Ptrofs.unsigned_range_2. }
+    rewrite (Ptrofs.unsigned_repr (Int64.unsigned _)).
+    2:{ change Ptrofs.max_unsigned with Int64.max_unsigned.
+        apply Int64.unsigned_range_2. }
+    apply Ptrofs.eqm_samerepr.
+    rewrite <- Ptrofs.eqm64; et.
+    apply Int64.eqm_unsigned_repr.
+  Qed.
 
 End AUX.
 
@@ -197,118 +193,6 @@ Section RULES.
   Context `{@GRA.inG allocatedRA Σ}.
   Context `{@GRA.inG blocksizeRA Σ}.
   Context `{@GRA.inG blockaddressRA Σ}.
-
-  (* Lemma capture_slide *)
-  (*     vaddr m i k *)
-  (*   : *)
-  (*     vaddr (≃_m) i ⊢ (Val.addl vaddr (Vptrofs k)) (≃_m) (Ptrofs.add i k). *)
-  (* Proof. *)
-  (*   unfold captured_to; des_ifs. *)
-  (*   - unfold Val.addl in *. des_ifs. iIntros "%". iPureIntro. clarify. *)
-  (*     unfold Vptrofs in Heq1. des_ifs. *)
-  (*     unfold Ptrofs.add, Ptrofs.of_int64, Ptrofs.to_int64, Int64.add. *)
-  (*     rewrite (Ptrofs.unsigned_repr). *)
-  (*     2:{ change Ptrofs.max_unsigned with Int64.max_unsigned. *)
-  (*         apply Int64.unsigned_range_2. } *)
-  (*     rewrite (Int64.unsigned_repr (Ptrofs.unsigned k)). *)
-  (*     2:{ change Int64.max_unsigned with Ptrofs.max_unsigned. *)
-  (*         apply Ptrofs.unsigned_range_2. } *)
-  (*     apply Ptrofs.eqm_repr_eq. *)
-  (*     rewrite (Ptrofs.unsigned_repr). *)
-  (*     2:{ change Ptrofs.max_unsigned with Int64.max_unsigned. *)
-  (*         apply Int64.unsigned_range_2. } *)
-  (*     rewrite <- Ptrofs.eqm64; et. *)
-  (*     apply Int64.eqm_unsigned_repr. *)
-  (*   - unfold Val.addl in *. des_ifs. unfold Vptrofs in *. des_ifs. *)
-  (*     iIntros "[a b]". iDestruct "b" as (a) "[b %]". *)
-  (*     iFrame. iExists _. iFrame. iPureIntro. des. clarify. split; et. *)
-  (*     rewrite Ptrofs.of_int64_to_int64; et. *)
-  (*     do 2 rewrite Ptrofs.sub_add_opp. do 2 rewrite Ptrofs.add_assoc. *)
-  (*     rewrite (Ptrofs.add_commut k). split; et. *)
-  (* Qed. *)
-
-  (* Lemma capture_unique *)
-  (*     vaddr m i j *)
-  (*   : *)
-  (*     vaddr (≃_m) i ** vaddr (≃_m) j ⊢ ⌜i = j⌝. *)
-  (* Proof. *)
-  (*   iIntros "[A B]". unfold captured_to. des_ifs.  *)
-  (*   - iDestruct "A" as "%". *)
-  (*     iDestruct "B" as "%". *)
-  (*     iPureIntro. clarify. *)
-  (*   - iDestruct "A" as "[A a]". *)
-  (*     iDestruct "B" as "[B b]". *)
-  (*     iDestruct "a" as (a) "[a %]". *)
-  (*     iDestruct "b" as (n) "[b %]". *)
-  (*     des. iCombine "a b" as "c". iOwnWf "c" as wfc. *)
-  (*     ur in wfc. ur in wfc. *)
-  (*     specialize (wfc (blk m)). unfold _has_base in wfc. *)
-  (*     des_ifs. iPureIntro. *)
-  (*     assert (Ptrofs.sub j x0 = Ptrofs.sub i x0). *)
-  (*     { rewrite Heq0. rewrite Heq. f_equal. apply proof_irr. } *)
-  (*     apply (f_equal (Ptrofs.add x0)) in H3. *)
-  (*     do 2 rewrite Ptrofs.sub_add_opp in H3. *)
-  (*     do 2 rewrite (Ptrofs.add_permut x0) in H3. *)
-  (*     rewrite Ptrofs.add_neg_zero in H3. *)
-  (*     do 2 rewrite Ptrofs.add_zero in H3. et. *)
-  (* Qed. *)
-
-  (* Lemma capture_dup *)
-  (*     vaddr m i *)
-  (*   : *)
-  (*     vaddr (≃_m) i ⊢ vaddr (≃_m) i ** vaddr (≃_m) i. *)
-  (* Proof. *)
-  (*   iIntros "A". unfold captured_to. des_ifs; et. *)
-  (*   iDestruct "A" as "[A B]". *)
-  (*   iDestruct "B" as (a) "[B %]". *)
-  (*   des. clarify. *)
-  (*   set (_has_size (blk m) (sz m)) at 1. *)
-  (*   replace c with ((_has_size (blk m) (sz m)) ⋅ (_has_size (blk m) (sz m))). *)
-  (*   2:{ unfold c. ur. apply func_ext. i. ur. des_ifs. unfold _has_size in Heq. des_ifs. } *)
-  (*   clear c. *)
-  (*   iDestruct "A" as "[B1 B2]". *)
-  (*   iFrame. *)
-  (*   replace (_has_base (blk m) a) with ((_has_base (blk m) a) ⋅ (_has_base (blk m) a)). *)
-  (*   2:{ ur. apply func_ext. i. ur. des_ifs. unfold _has_base in Heq. des_ifs. } *)
-  (*   iDestruct "B" as "[B1 B2]". *)
-  (*   iSplitL "B1". *)
-  (*   { iExists _. iFrame. ss. } *)
-  (*   { iExists _. iFrame. ss. } *)
-  (* Qed. *)
-
-  (* Lemma capture_trans *)
-  (*     vaddr m i j *)
-  (*   : *)
-  (*     vaddr (≃_m) i ** Vptrofs i (≃_m) j *)
-  (*     ⊢ vaddr (≃_m) j. *)
-  (* Proof. *)
-  (*   iIntros "[A B]". unfold captured_to. *)
-  (*   des_ifs. *)
-  (*   - iDestruct "A" as "%". *)
-  (*     iDestruct "B" as "%". *)
-  (*     clarify. unfold Vptrofs in Heq0. des_ifs. *)
-  (*     rewrite Ptrofs.of_int64_to_int64; et. *)
-  (*   - iDestruct "A" as "[A C]". *)
-  (*     iDestruct "B" as "%". *)
-  (*     iDestruct "C" as (a) "[C %]". *)
-  (*     des. clarify. iFrame. iExists _. iFrame. *)
-  (*     unfold Vptrofs in Heq. des_ifs. *)
-  (*     rewrite Ptrofs.of_int64_to_int64; et. *)
-  (* Qed. *)
-
-  (* Lemma capture_refl *)
-  (*     m i vaddr *)
-  (*   : *)
-  (*     vaddr (≃_m) i ⊢ (Vptrofs i) (≃_m) i. *)
-  (* Proof. *)
-  (*   iIntros "A". *)
-  (*   unfold captured_to. des_ifs. *)
-  (*   - unfold Vptrofs in Heq0. des_ifs. iDestruct "A" as "%". clarify. *)
-  (*     rewrite Ptrofs.of_int64_to_int64; et. *)
-  (*   - unfold Vptrofs in Heq. des_ifs. iDestruct "A" as "[A B]". *)
-  (*     iDestruct "B" as (a) "[B %]". des. clarify. *)
-  (*     rewrite Ptrofs.of_int64_to_int64; et. *)
-  (* Qed. *)
 
   Lemma _has_size_dup
       b s
@@ -322,46 +206,57 @@ Section RULES.
     iDestruct "A" as "[? ?]". iFrame.
   Qed.
 
+  Lemma _has_base_dup
+      b s
+    :
+      OwnM (_has_base b s) ⊢ OwnM (_has_base b s) ** OwnM (_has_base b s).
+  Proof.
+    iIntros "A".
+    set (_has_base _ _) at 1.
+    replace c with ((_has_base b s) ⋅ (_has_base b s)).
+    2:{ unfold c. ur. apply func_ext. i. ur. des_ifs. unfold _has_base in Heq. des_ifs. }
+    iDestruct "A" as "[? ?]". iFrame.
+  Qed.
+
+  Lemma _has_base_unique
+      b s0 s1
+    :
+      OwnM (_has_base b s0 ⋅ _has_base b s1) ⊢ ⌜s0 = s1⌝.
+  Proof.
+    iIntros "C".
+    iOwnWf "C" as wfc. iPureIntro.
+    ur in wfc. specialize (wfc b).
+    ur in wfc. unfold _has_base in wfc. des_ifs.
+  Qed.
+
   Lemma _has_offset_slide
       vaddr m ofs k
     :
       vaddr ⊨ m # ofs ⊢ Val.addl vaddr (Vptrofs k) ⊨ m # (Ptrofs.add ofs k).
   Proof.
     destruct m. destruct blk0; cycle 1.
-    { unfold _has_offset. ss. des_ifs.
-      - iIntros "[A B]".
+    - unfold _has_offset. ss. des_ifs.
+      + iIntros "[A B]".
         iDestruct "B" as (a) "[B %]".
-        iFrame. iExists a. iFrame. admit "true".
-      - iIntros "[A %]". des; clarify. }
-    admit "use existing proof".
-    (* iIntros "A". *)
-    (* unfold _has_offset. *)
-    (* des_ifs; try solve [iDestruct "A" as "[A %]"; clarify].  *)
-    (* - iDestruct "A" as "[? A]". *)
-    (*   iFrame. *)
-    (*   replace (Vptr (blk m) (Ptrofs.add ofs k)) *)
-    (*     with (Val.addl (Vptr (blk m) ofs) (Vptrofs k)). *)
-    (*   2:{ ss. des_ifs. unfold Vptrofs in *. des_ifs. rewrite Ptrofs.of_int64_to_int64; et. } *)
-    (*   unfold Val.addl in Heq0. des_ifs. *)
-    (*   unfold Vptrofs in Heq1. des_ifs. *)
-    (*   replace (Ptrofs.of_int64 (Int64.add i (Ptrofs.to_int64 k))) *)
-    (*     with (Ptrofs.add (Ptrofs.of_int64 i) k). *)
-    (*   2:{ unfold Ptrofs.add, Ptrofs.of_int64, Int64.add, Ptrofs.to_int64. *)
-    (*       rewrite (Int64.unsigned_repr (Ptrofs.unsigned _)). *)
-    (*       2:{ change Int64.max_unsigned with Ptrofs.max_unsigned. *)
-    (*           apply Ptrofs.unsigned_range_2. } *)
-    (*       rewrite Ptrofs.unsigned_repr. *)
-    (*       2:{ change Ptrofs.max_unsigned with Int64.max_unsigned. *)
-    (*           apply Int64.unsigned_range_2. } *)
-    (*       apply Ptrofs.eqm_samerepr. *)
-    (*       rewrite <- Ptrofs.eqm64; et. *)
-    (*       apply Int64.eqm_unsigned_repr_r. *)
-    (*       apply Int64.eqm_refl. } *)
-    (*   iApply capture_slide. et. *)
-    (* - iDestruct "A" as "[A %]". *)
-    (*   iFrame. iPureIntro. des. clarify. *)
-    (*   ss. des_ifs. unfold Vptrofs in *. des_ifs. *)
-    (*   split; et. rewrite Ptrofs.of_int64_to_int64; et. *)
+        iFrame. iExists a. iFrame.
+        iPureIntro.
+        des. split; clarify. rewrite <- Ptrofs.sub_add_l. f_equal.
+        unfold Val.addl, Vptrofs in *.
+        des_ifs. rewrite ptrofs_int64_add; et.
+      + iIntros "[A %]". des; clarify.
+    - iIntros "A".
+      unfold _has_offset.
+      des_ifs; try solve [iDestruct "A" as "[A %]"; clarify].
+      + iDestruct "A" as "[? A]". iFrame.
+        iDestruct "A" as (a) "[? %]". iExists _. iFrame.
+        iPureIntro. des. clarify. split; clarify.
+        rewrite <- Ptrofs.sub_add_l. f_equal.
+        unfold Val.addl, Vptrofs in *.
+        des_ifs. rewrite ptrofs_int64_add; et.
+      + iDestruct "A" as "[A %]".
+        iFrame. iPureIntro. des. clarify.
+        ss. des_ifs. unfold Vptrofs in *. des_ifs.
+        split; et. rewrite Ptrofs.of_int64_to_int64; et.
   Qed.
 
   Lemma _has_offset_unique
@@ -374,8 +269,6 @@ Section RULES.
     des_ifs; try solve [iDestruct "A" as "[A %]"; clarify]. 
     - iDestruct "A" as "[_ A]".
       iDestruct "B" as "[_ B]".
-      (* iDestruct "A" as "[A A1]". *)
-      (* iDestruct "B" as "[B B1]". *)
       iDestruct "A" as (a) "[A1 %]".
       iDestruct "B" as (a0) "[B1 %]".
       des. clarify.
@@ -386,6 +279,21 @@ Section RULES.
     - iDestruct "A" as "[A %]".
       iDestruct "B" as "[B %]".
       des. clarify.
+  Qed.
+
+  Lemma _offset_dup
+      vaddr m ofs
+    :
+      vaddr ⊨m# ofs ⊢ vaddr ⊨m# ofs ** vaddr ⊨m# ofs.
+  Proof.
+    iIntros "[A' A]".
+    unfold _has_offset.
+    iPoseProof (_has_size_dup with "A'") as "[? ?]".
+    des_ifs; try solve [iDestruct "A" as "%"; clarify].
+    - iDestruct "A" as (a) "[A %]".
+      iPoseProof (_has_base_dup with "A") as "[A B]".
+      iFrame. iSplitL "A"; iExists _; iFrame; clarify.
+    - iDestruct "A" as "%". iFrame. ss.
   Qed.
 
   Lemma offset_slide
@@ -413,17 +321,14 @@ Section RULES.
     iApply _has_offset_unique; et.
   Qed.
 
-  Lemma _offset_dup
-      vaddr m ofs
+  Lemma _points_to_ownership
+      b ofs mvs q0 q1
     :
-      vaddr ⊨m# ofs ⊢ vaddr ⊨m# ofs ** vaddr ⊨m# ofs.
+      _points_to b ofs mvs (q0 + q1) = (_points_to b ofs mvs q0) ⋅ (_points_to b ofs mvs q1).
   Proof.
-    iIntros "[A B]".
-    unfold _has_offset.
-    iPoseProof (_has_size_dup with "A") as "[? ?]".
-    des_ifs.
-    - (* iPoseProof (_dup with "B") as "[? ?]". iFrame. *) admit "base dup".
-    - iDestruct "B" as "%". iFrame. ss.
+    unfold _points_to. unfold Auth.white. ur. ur. ur.
+    f_equal. ss. apply func_ext. i. apply func_ext. i. ur.
+    unfold __points_to. des_ifs.
   Qed.
 
   Lemma points_to_ownership
@@ -431,240 +336,141 @@ Section RULES.
     : 
       ⊢ vaddr (↦_ m, q0 + q1) mvs ∗-∗ (vaddr (↦_ m, q0) mvs ** vaddr (↦_ m, q1) mvs).
   Proof.
-    (* iIntros. iSplit. *)
-    (* - iIntros "A". unfold points_to. *)
-    (*   iDestruct "A" as "[B A]". *)
-    (*   iPoseProof (_has_size_dup with "B") as "[Y T]". *)
-    (*   des_ifs; iDestruct "A" as (ofs) "[[[A B] %] %]"; des; clarify. *)
-    (*   + unfold _has_offset. des_ifs. iDestruct "B" as "[? %]". *)
-    (*     clarify. *)
-    (*   + iPoseProof (_offset_dup with "B") as "[C D]". *)
-    (*     replace (_points_to (blk m) (Ptrofs.unsigned ofs) mvs (q0+q1)%Qp) *)
-    (*       with ((_points_to (blk m) (Ptrofs.unsigned ofs) mvs q0) *)
-    (*             ⋅ (_points_to (blk m) (Ptrofs.unsigned ofs) mvs q1)). *)
-    (*     2:{ unfold _points_to. unfold Auth.white. ur. ur. ur. *)
-    (*         f_equal. apply func_ext. i. apply func_ext. i. ur. *)
-    (*         unfold __points_to. des_ifs. } *)
-    (*     iDestruct "A" as "[A B]". *)
-    (*     iSplitL "A Y D"; iFrame; iExists _; iFrame; et. *)
-    (*   + iPoseProof (_offset_dup with "B") as "[C D]". *)
-    (*     replace (_points_to (blk m) (Ptrofs.unsigned ofs) mvs (q0+q1)%Qp) *)
-    (*       with ((_points_to (blk m) (Ptrofs.unsigned ofs) mvs q0) *)
-    (*             ⋅ (_points_to (blk m) (Ptrofs.unsigned ofs) mvs q1)). *)
-    (*     2:{ unfold _points_to. unfold Auth.white. ur. ur. ur. *)
-    (*         f_equal. apply func_ext. i. apply func_ext. i. ur. *)
-    (*         unfold __points_to. des_ifs. } *)
-    (*     iDestruct "A" as "[A B]". *)
-    (*     iSplitL "A Y D"; iFrame; iExists _; iFrame; et. *)
-    (* - iIntros "A". unfold points_to. *)
-    (*   iDestruct "A" as "[[A B] [C D]]". *)
-    (*   iDestruct "B" as (ofs0) "[[[E G] %] F]". *)
-    (*   iDestruct "D" as (ofs1) "[[[H I] %] J]". *)
-    (*   iCombine "I G" as "T". *)
-    (*   iPoseProof (_has_offset_unique with "T") as "%". *)
-    (*   clarify. *)
-    (*   des_ifs; try solve [iDestruct "F" as "%"; clarify]. *)
-    (*   + unfold _has_offset. des_ifs. iDestruct "T" as "[[_ %] _]". *)
-    (*     clarify. *)
-    (*   + iSplitL "A"; ss. iDestruct "T" as "[T T']". *)
-    (*     iExists _. iFrame. *)
-    (*     replace (_points_to (blk m) (Ptrofs.unsigned ofs0) mvs (q0+q1)%Qp) *)
-    (*       with ((_points_to (blk m) (Ptrofs.unsigned ofs0) mvs q0) *)
-    (*             ⋅ (_points_to (blk m) (Ptrofs.unsigned ofs0) mvs q1)). *)
-    (*     2:{ unfold _points_to. unfold Auth.white. ur. ur. ur. *)
-    (*         f_equal. apply func_ext. i. apply func_ext. i. ur. *)
-    (*         unfold __points_to. des_ifs. } *)
-    (*     iCombine "E H" as "?". iFrame. ss. *)
-    (*   + iSplitL "A"; ss. iDestruct "T" as "[T T']". *)
-    (*     iExists _. iFrame. *)
-    (*     replace (_points_to (blk m) (Ptrofs.unsigned ofs0) mvs (q0+q1)%Qp) *)
-    (*       with ((_points_to (blk m) (Ptrofs.unsigned ofs0) mvs q0) *)
-    (*             ⋅ (_points_to (blk m) (Ptrofs.unsigned ofs0) mvs q1)). *)
-    (*     2:{ unfold _points_to. unfold Auth.white. ur. ur. ur. *)
-    (*         f_equal. apply func_ext. i. apply func_ext. i. ur. *)
-    (*         unfold __points_to. des_ifs. } *)
-    (*     iCombine "E H" as "?". iFrame. ss. *)
-    admit "".
+    iIntros. iSplit.
+    - iIntros "A". unfold points_to.
+      destruct (blk m); try solve [iDestruct "A" as "%"; clarify].
+      iDestruct "A" as "[B A]".
+      iPoseProof (_has_size_dup with "B") as "[? ?]". iFrame.
+      des_ifs; iDestruct "A" as (ofs) "[[[B A] %] %]"; des; clarify.
+      + unfold _has_offset. des_ifs. iDestruct "A" as "[? %]"; clarify.
+      + iPoseProof (_offset_dup with "A") as "[C D]".
+        rewrite _points_to_ownership.
+        iDestruct "B" as "[A B]".
+        iSplitL "A C"; iExists _; iFrame; et.
+      + iPoseProof (_offset_dup with "A") as "[C D]".
+        rewrite _points_to_ownership.
+        iDestruct "B" as "[A B]".
+        iSplitL "A C"; iExists _; iFrame; et.
+    - iIntros "A". unfold points_to.
+      iDestruct "A" as "[B A]".
+      destruct (blk m); try solve [iDestruct "A" as "%"; clarify]. 
+      iDestruct "A" as "[? A]". iDestruct "B" as "[? B]". iFrame.
+      des_ifs; iDestruct "A" as (ofs0) "[[[A A'] %] %]"; des; clarify.
+      + unfold _has_offset. des_ifs. iDestruct "A'" as "[_ %]". clarify.
+      + iDestruct "B" as (ofs1) "[[[B B'] %] %]"; des; clarify.
+        iCombine "B' A'" as "C".
+        iPoseProof (_has_offset_unique with "C") as "%". iDestruct "C" as "[_ C]". clarify.
+        iCombine "B A" as "?".
+        rewrite <- _points_to_ownership.
+        iExists _. iFrame. iPureIntro. nia.
+      + iDestruct "B" as (ofs1) "[[[B B'] %] %]"; des; clarify.
+        iCombine "B' A'" as "C".
+        iPoseProof (_has_offset_unique with "C") as "%". iDestruct "C" as "[_ C]". clarify.
+        iCombine "B A" as "?".
+        rewrite <- _points_to_ownership.
+        iExists _. iFrame. iPureIntro. nia.
   Qed.
 
-  (* Lemma _allocated_disjoint *)
-  (*     m0 m1 tg0 tg1 q *)
-  (*   :  *)
-  (*     live_ 1# (m0, tg0) ** live_ q# (m1, tg1) *)
-  (*     ⊢ ⌜m0 #^ m1⌝%I.  *)
-  (* Proof. *)
-  (*   unfold metadata_alive. *)
-  (*   iIntros "[[A _][B _]]". *)
-  (*   iCombine "A B" as "C". *)
-  (*   iOwnWf "C" as wfc. iPureIntro. *)
-  (*   unfold _allocated_with, __allocated_with in wfc. *)
-  (*   ur in wfc. ur in wfc. specialize (wfc (blk m0)). *)
-  (*   ur in wfc. des_ifs. *)
-  (*   apply Qp_not_add_le_l in wfc. clarify. *)
-  (* Qed. *)
-
-  (* Lemma _allocated_ownership *)
-  (*     m tg q0 q1 *)
-  (*   :  *)
-  (*     ⊢ live_ (q0 + q1)%Qp# (m, tg) ∗-∗ (live_ q0# (m, tg) ** live_ q1# (m, tg)). *)
-  (* Proof. *)
-  (*   iIntros. iSplit. *)
-  (*   - iIntros "A". *)
-  (*     unfold metadata_alive. *)
-  (*     iDestruct "A" as "[A A']". *)
-  (*     iPoseProof (_has_size_dup with "A'") as "[? ?]". *)
-  (*     iFrame. *)
-  (*     replace (_allocated_with (blk m) tg (q0 + q1)%Qp) *)
-  (*       with ((_allocated_with (blk m) tg q0) ⋅ (_allocated_with (blk m) tg q1)).  *)
-  (*     2:{ unfold _allocated_with. unfold Auth.white. ur. ur. *)
-  (*         f_equal. apply func_ext. i. unfold __allocated_with. *)
-  (*         ur. des_ifs. } *)
-  (*     iDestruct "A" as "[? ?]". *)
-  (*     iFrame. *)
-  (*   - iIntros "A". *)
-  (*     unfold metadata_alive. *)
-  (*     iDestruct "A" as "[[A B] [A' B']]". *)
-  (*     iFrame. *)
-  (*     replace (_allocated_with (blk m) tg (q0 + q1)%Qp) *)
-  (*       with ((_allocated_with (blk m) tg q0) ⋅ (_allocated_with (blk m) tg q1)).  *)
-  (*     2:{ unfold _allocated_with. unfold Auth.white. ur. ur. *)
-  (*         f_equal. apply func_ext. i. unfold __allocated_with. *)
-  (*         ur. des_ifs. } *)
-  (*     iSplitL "A"; iFrame. *)
-  (* Qed. *)
+  Lemma _allocated_with_ownership
+      b tg q0 q1
+    :
+      _allocated_with b tg (q0 + q1) = (_allocated_with b tg q0) ⋅ (_allocated_with b tg q1).
+  Proof.
+    unfold _allocated_with. unfold Auth.white. ur. ur. ur.
+    f_equal. ss. apply func_ext. i.
+    unfold __allocated_with. des_ifs.
+  Qed.
 
   Lemma offset_ownership
       vaddr m tg q0 q1 ofs
     :
       ⊢ vaddr (⊨_ m, tg, (q0 + q1)%Qp) ofs  ∗-∗ (vaddr (⊨_ m, tg, q0) ofs ** vaddr (⊨_ m, tg, q1) ofs).
   Proof.
-    destruct m. destruct blk0; cycle 1.
-    { unfold has_offset. ss. iSplit; iIntros "%"; des; clarify. }
-    (* iIntros. iSplit. *)
-    (* - iIntros "A". unfold has_offset. *)
-    (*   iDestruct "A" as "[A A']". *)
-    (*   iPoseProof (_allocated_ownership with "A") as "[? ?]". *)
-    (*   iPoseProof (_offset_dup with "A'") as "[? ?]". *)
-    (*   iFrame. *)
-    (* - iIntros "A". unfold has_offset. *)
-    (*   iDestruct "A" as "[[A B] [A' B']]". *)
-    (*   iCombine "A A'" as "A". *)
-    (*   iPoseProof (_allocated_ownership with "A") as "?". *)
-    (*   iFrame. *)
-    admit "".
+    iIntros. iSplit.
+    - iIntros "A". unfold has_offset.
+      destruct (blk m); try solve [iDestruct "A" as "%"; clarify].
+      rewrite _allocated_with_ownership.
+      iDestruct "A" as "[[? ?] A]".
+      iPoseProof (_offset_dup with "A") as "[? ?]".
+      iFrame.
+    - iIntros "A". unfold has_offset.
+      iDestruct "A" as "[A B]".
+      destruct (blk m); try solve [iDestruct "A" as "%"; clarify].
+      iDestruct "A" as "[A ?]".
+      iDestruct "B" as "[B ?]".
+      iCombine "A B" as "?".
+      rewrite _allocated_with_ownership. iFrame.
+  Qed.
+
+  Lemma _points_to_content
+      b ofs mvs0 mvs1 q
+    :
+      _points_to b ofs (mvs0 ++ mvs1) q = (_points_to b ofs mvs0 q) ⋅ (_points_to b (ofs + length mvs0) mvs1 q).
+  Proof.
+    unfold _points_to. unfold Auth.white. ur. ur. ur.
+    f_equal. ss. apply func_ext. i. apply func_ext. i. ur.
+    unfold __points_to.
+    destruct dec; ss;
+    destruct Coqlib.zle; ss;
+    destruct Coqlib.zlt; ss;
+    try destruct Coqlib.zle; ss;
+    try destruct Coqlib.zlt; ss;
+    try destruct Coqlib.zlt; ss;
+    des_ifs; try rewrite app_length in *; try nia;
+    try solve [rewrite nth_error_app1 in *; try nia; clarify
+              |rewrite nth_error_app2 in *; try nia;
+               replace (Z.to_nat _) with ((Z.to_nat (x0 - ofs)) - length mvs0)%nat in * by nia;
+               clarify].
   Qed.
 
   Lemma points_to_split
       vaddr mvs0 mvs1 m q
     : 
-      vaddr (↦_ m , q) (mvs0 ++ mvs1)
-      ⊢ vaddr (↦_ m , q) mvs0 ** (Val.addl vaddr (Vptrofs (Ptrofs.repr (length mvs0))) (↦_m,q) mvs1).
+      vaddr (↦_m,q) (mvs0 ++ mvs1)
+      ⊢ vaddr (↦_m,q) mvs0 ** (Val.addl vaddr (Vptrofs (Ptrofs.repr (length mvs0))) (↦_m,q) mvs1).
   Proof.
-    (* iIntros "A". unfold points_to. *)
-    (* iDestruct "A" as "[A B]". *)
-    (* des_ifs; try solve [iDestruct "B" as (ofs) "[_ %]"; clarify]. *)
-    (* - iDestruct "B" as (ofs) "[B %]". *)
-    (*   unfold _has_offset. des_ifs. iDestruct "B" as "[[_ [_ %]] _]". clarify. *)
-    (* - iDestruct "B" as (ofs) "[[[B C] %] %]". *)
-    (*   des. clarify. *)
-    (*   iPoseProof (_has_size_dup with "A") as "[A A']". *)
-    (*   iPoseProof (_offset_dup with "C") as "[C C']". *)
-    (*   replace (_points_to (blk m) (Ptrofs.unsigned ofs) (mvs0 ++ mvs1) q) *)
-    (*     with ((_points_to (blk m) (Ptrofs.unsigned ofs) mvs0 q) *)
-    (*           ⋅ (_points_to (blk m) (Ptrofs.unsigned ofs + length mvs0) mvs1 q)). *)
-    (*   2:{ unfold _points_to. unfold Auth.white. ur. ur. *)
-    (*       f_equal. apply func_ext. i. ur. apply func_ext. i. ur. *)
-    (*       unfold __points_to. *)
-    (*       destruct dec; ss; *)
-    (*       destruct Coqlib.zle; ss; *)
-    (*       destruct Coqlib.zlt; ss; *)
-    (*       try destruct Coqlib.zle; ss; *)
-    (*       try destruct Coqlib.zlt; ss; *)
-    (*       try destruct Coqlib.zlt; ss; *)
-    (*       des_ifs; rewrite app_length in *; try nia; *)
-    (*       try solve [rewrite nth_error_app1 in *; try nia; clarify *)
-    (*                 |rewrite nth_error_app2 in *; try nia; *)
-    (*                  replace (Z.to_nat _) with *)
-    (*                   ((Z.to_nat (x0 - Ptrofs.unsigned ofs)) - length mvs0)%nat in Heq3 by nia; *)
-    (*                     clarify]. } *)
-    (*   iDestruct "B" as "[B B']". *)
-    (*   iSplitL "A B C". *)
-    (*   { iSplitL "A"; ss. iExists _. iFrame. iPureIntro. rewrite app_length in *. nia. } *)
-    (*   iSplitL "A'"; ss. iExists (Ptrofs.repr (Ptrofs.unsigned ofs + length mvs0)). *)
-    (*   des_ifs. *)
-    (*   rewrite Ptrofs.unsigned_repr.  *)
-    (*   2:{ rewrite app_length in *. destruct ofs; ss. nia. } *)
-    (*   iFrame. *)
-    (*   iSplitL "C'". *)
-    (*   { unfold _has_offset. des_ifs. iDestruct "C'" as "[? C]". iFrame. *)
-    (*     iPoseProof ((capture_slide _ _ _ (Ptrofs.repr (length mvs0))) with "C") as "C". *)
-    (*     unfold Val.addl. des_ifs_safe. unfold Vptrofs in *. *)
-    (*     des_ifs. rewrite Ptrofs.of_int64_to_int64; et.  *)
-    (*     unfold Ptrofs.add, Int64.add, Ptrofs.to_int64, Ptrofs.of_int64. *)
-    (*     rewrite app_length in *. *)
-    (*     destruct ofs; ss. *)
-    (*     destruct i; ss. *)
-    (*     rewrite Ptrofs.unsigned_repr; try nia. *)
-    (*     rewrite (Int64.unsigned_repr (length _)). *)
-    (*     2:{ change Int64.max_unsigned with Ptrofs.max_unsigned. nia. } *)
-    (*     iDestruct "C" as "[? C]". iFrame. *)
-    (*     iDestruct "C" as (a) "[C %]". des. *)
-    (*     iSplit. *)
-    (*     2:{ iPureIntro. nia. } *)
-    (*     iExists _. iFrame. iPureIntro. *)
-    (*     split; et. rewrite Int64.unsigned_repr; try nia. *)
-    (*     rewrite Ptrofs.unsigned_repr in *; try nia. *)
-    (*     2:{ change Int64.max_unsigned with Ptrofs.max_unsigned. nia. } *)
-    (*     et. } *)
-    (*   iPureIntro. rewrite app_length in *. *)
-    (*   unfold Vptrofs in *. des_ifs. unfold Int64.add, Ptrofs.to_int64. *)
-    (*   destruct i; ss; destruct ofs; ss.       *)
-    (*   rewrite Ptrofs.unsigned_repr; try nia. *)
-    (*   rewrite (Int64.unsigned_repr (length _)). *)
-    (*   2:{ change Int64.max_unsigned with Ptrofs.max_unsigned. nia. } *)
-    (*   rewrite Int64.unsigned_repr; try nia. *)
-    (*   change Int64.max_unsigned with Ptrofs.max_unsigned. nia. *)
-    (* - iDestruct "B" as (ofs) "[[[B C] %] %]". *)
-    (*   iPoseProof (_has_size_dup with "A") as "[A A']". *)
-    (*   iPoseProof (_offset_dup with "C") as "[C C']". *)
-    (*   replace (_points_to (blk m) (Ptrofs.unsigned ofs) (mvs0 ++ mvs1) q) *)
-    (*     with ((_points_to (blk m) (Ptrofs.unsigned ofs) mvs0 q) *)
-    (*           ⋅ (_points_to (blk m) (Ptrofs.unsigned ofs + length mvs0) mvs1 q)). *)
-    (*   2:{ unfold _points_to. unfold Auth.white. ur. ur. *)
-    (*       f_equal. apply func_ext. i. ur. apply func_ext. i. ur. *)
-    (*       unfold __points_to. *)
-    (*       destruct dec; ss; *)
-    (*       destruct Coqlib.zle; ss; *)
-    (*       destruct Coqlib.zlt; ss; *)
-    (*       try destruct Coqlib.zle; ss; *)
-    (*       try destruct Coqlib.zlt; ss; *)
-    (*       try destruct Coqlib.zlt; ss; *)
-    (*       des_ifs; rewrite app_length in *; try nia; *)
-    (*       try solve [rewrite nth_error_app1 in *; try nia; clarify *)
-    (*                 |rewrite nth_error_app2 in *; try nia; *)
-    (*                  replace (Z.to_nat _) with *)
-    (*                   ((Z.to_nat (x0 - Ptrofs.unsigned ofs)) - length mvs0)%nat in Heq3 by nia; *)
-    (*                     clarify]. } *)
-    (*   iDestruct "B" as "[B B']". *)
-    (*   iSplitL "A B C". *)
-    (*   { iSplitL "A"; ss. iExists _. iFrame. iPureIntro. rewrite app_length in *. nia. } *)
-    (*   iSplitL "A'"; ss. iExists (Ptrofs.repr (Ptrofs.unsigned ofs + length mvs0)). *)
-    (*   des_ifs. *)
-    (*   rewrite Ptrofs.unsigned_repr.  *)
-    (*   2:{ rewrite app_length in *. destruct ofs; ss. nia. } *)
-    (*   iFrame. *)
-    (*   iSplitL "C'". *)
-    (*   { unfold _has_offset. iDestruct "C'" as "[? %]". iFrame. *)
-    (*     iPureIntro. des. clarify. rewrite app_length in *. *)
-    (*     split; try nia. *)
-    (*     unfold Vptrofs in *. *)
-    (*     des_ifs. rewrite Ptrofs.of_int64_to_int64; et.  *)
-    (*     unfold Ptrofs.add. *)
-    (*     rewrite Ptrofs.unsigned_repr. *)
-    (*     2:{ destruct i; ss. nia. } et. } *)
-    (*   iPureIntro. rewrite app_length in *. *)
-    (*   unfold Vptrofs in *. des_ifs. nia. *)
-    admit "".
+    iIntros "A". unfold points_to.
+    destruct (blk m); try solve [iDestruct "A" as "%"; clarify].
+    iDestruct "A" as "[B A]".
+    iPoseProof (_has_size_dup with "B") as "[? ?]". iFrame.
+    des_ifs; iDestruct "A" as (ofs) "[[[B A] %] %]"; des; clarify.
+    - unfold _has_offset. des_ifs. iDestruct "A" as "[? %]"; clarify.
+    - rewrite _points_to_content.
+      iPoseProof (_offset_dup with "A") as "[? A]".
+      iDestruct "B" as "[? B]".
+      rewrite <- Heq.
+      iSplitR "A B"; iExists _; iFrame.
+      + iPureIntro. rewrite app_length in *. nia.
+      + rewrite app_length in *.
+        assert (X: Ptrofs.unsigned ofs + length mvs0 = Ptrofs.unsigned (Ptrofs.add ofs (Ptrofs.repr (length mvs0)))).
+        { unfold Ptrofs.add. destruct ofs. ss.
+          rewrite (Ptrofs.unsigned_repr (length _)); try nia.
+          rewrite (Ptrofs.unsigned_repr); et. nia. }
+        rewrite X. iFrame. iSplit; iSplit.
+        { iApply _has_offset_slide. et. }
+        all: iPureIntro; try nia.
+        unfold Val.addl, Vptrofs in *. des_ifs.
+        assert (X0: Int64.unsigned i + length mvs0 = Int64.unsigned (Int64.add i (Ptrofs.to_int64 (Ptrofs.repr (length mvs0))))).
+        { unfold Int64.add, Ptrofs.to_int64. destruct i. ss.
+          rewrite (Ptrofs.unsigned_repr (length _)); try nia.
+          change Ptrofs.max_unsigned with Int64.max_unsigned in *.
+          rewrite (Int64.unsigned_repr (length _)); try nia.
+          rewrite (Int64.unsigned_repr); et. nia. }
+        rewrite <- X0. nia.
+    - rewrite _points_to_content.
+      iPoseProof (_offset_dup with "A") as "[? A]".
+      iDestruct "B" as "[? B]".
+      rewrite <- Heq.
+      iSplitR "A B"; iExists _; iFrame.
+      + iPureIntro. rewrite app_length in *. nia.
+      + rewrite app_length in *.
+        assert (X: Ptrofs.unsigned ofs + length mvs0 = Ptrofs.unsigned (Ptrofs.add ofs (Ptrofs.repr (length mvs0)))).
+        { unfold Ptrofs.add. destruct ofs. ss.
+          rewrite (Ptrofs.unsigned_repr (length _)); try nia.
+          rewrite (Ptrofs.unsigned_repr); et. nia. }
+        rewrite X. iFrame. iSplit; try iSplit.
+        { iApply _has_offset_slide. et. }
+        all: iPureIntro; try nia.
   Qed.
 
   Lemma points_to_collect
@@ -673,223 +479,156 @@ Section RULES.
       vaddr (↦_m,q) mvs0 ** (Val.addl vaddr (Vptrofs (Ptrofs.repr (Z.of_nat (List.length mvs0)))) (↦_m,q) mvs1)
       ⊢ vaddr (↦_m,q) (mvs0 ++ mvs1).
   Proof.
-    (* iIntros "[A B]". unfold points_to. *)
-    (* iDestruct "A" as "[A' A]". *)
-    (* iDestruct "B" as "[B' B]". *)
-    (* iDestruct "A" as (ofs0) "[[[A C] %] H]". *)
-    (* iDestruct "B" as (ofs1) "[[[B D] %] J]". *)
-    (* des_ifs. *)
-    (* - iDestruct "H" as "%". *)
-    (*   iDestruct "J" as "%". *)
-    (*   rewrite <- Heq. *)
-    (*   iPoseProof (_offset_dup with "C") as "[C C']". *)
-    (*   iPoseProof ((_has_offset_slide _ _ _ (Ptrofs.repr (length mvs0))) with "C'") as "C'". *)
-    (*   iCombine "C' D" as "C'". *)
-    (*   iPoseProof (_has_offset_unique with "C'") as "%". *)
-    (*   clarify. *)
-    (*   iDestruct "C'" as "[C' _]". *)
-    (*   iCombine "A B" as "A". *)
-    (*   replace (Ptrofs.unsigned (Ptrofs.add ofs0 (Ptrofs.repr (length mvs0)))) *)
-    (*     with (Ptrofs.unsigned ofs0 + length mvs0). *)
-    (*   2:{ des. unfold Ptrofs.add. rewrite (Ptrofs.unsigned_repr (length _)). *)
-    (*       2:{ destruct ofs0; ss. nia. } *)
-    (*       rewrite Ptrofs.unsigned_repr. *)
-    (*       2:{ destruct ofs0; ss. nia. } et. } *)
-    (*   replace ((_points_to (blk m) (Ptrofs.unsigned ofs0) mvs0 q) *)
-    (*             ⋅ (_points_to (blk m) (Ptrofs.unsigned ofs0 + (length mvs0))) mvs1 q) *)
-    (*       with (_points_to (blk m) (Ptrofs.unsigned ofs0) (mvs0 ++ mvs1) q). *)
-    (*   2:{ unfold _points_to. unfold Auth.white. ur. ur. *)
-    (*       f_equal. ss. apply func_ext. i. ur. apply func_ext. i. ur. *)
-    (*       unfold __points_to. *)
-    (*       destruct dec; ss; *)
-    (*       destruct Coqlib.zle; ss; *)
-    (*       destruct Coqlib.zlt; ss; *)
-    (*       try destruct Coqlib.zle; ss; *)
-    (*       try destruct Coqlib.zlt; ss; *)
-    (*       try destruct Coqlib.zlt; ss; *)
-    (*       des_ifs; try rewrite app_length in *; try nia; *)
-    (*       try solve [rewrite nth_error_app1 in *; try nia; clarify *)
-    (*                 |rewrite nth_error_app2 in *; try nia; *)
-    (*                  replace (Z.to_nat _) with *)
-    (*                   ((Z.to_nat (x0 - Ptrofs.unsigned ofs0)) - length mvs0)%nat in Heq3 by nia; *)
-    (*                     clarify]. } *)
-    (*   iSplitL "A'"; ss. iExists _. iFrame. *)
-    (*   iPureIntro. des. *)
-    (*   unfold Vptrofs in *. des_ifs. *)
-    (*   unfold Ptrofs.add, Ptrofs.to_int64, Int64.add in *.  *)
-    (*   rewrite (Ptrofs.unsigned_repr (length mvs0)) in *. *)
-    (*   2,3,4: destruct ofs0; ss; nia. *)
-    (*   rewrite (Int64.unsigned_repr (length mvs0)) in *. *)
-    (*   2: change Int64.max_unsigned with Ptrofs.max_unsigned; *)
-    (*        destruct i; ss; nia. *)
-    (*   rewrite Ptrofs.unsigned_repr in *. *)
-    (*   2,3: destruct ofs0; ss; nia. *)
-    (*   rewrite (Int64.unsigned_repr) in *. *)
-    (*   2: change Int64.max_unsigned with Ptrofs.max_unsigned; *)
-    (*        destruct i; ss; nia. *)
-    (*   rewrite app_length in *. nia. *)
-    (* - iDestruct "H" as "%". *)
-    (*   iDestruct "J" as "%". *)
-    (*   rewrite <- Heq. *)
-    (*   iPoseProof (_offset_dup with "C") as "[C C']". *)
-    (*   iPoseProof ((_has_offset_slide _ _ _ (Ptrofs.repr (length mvs0))) with "C'") as "C'". *)
-    (*   iCombine "C' D" as "C'". *)
-    (*   iPoseProof (_has_offset_unique with "C'") as "%". *)
-    (*   clarify. *)
-    (*   iDestruct "C'" as "[C' _]". *)
-    (*   iCombine "A B" as "A". *)
-    (*   replace (Ptrofs.unsigned (Ptrofs.add ofs0 (Ptrofs.repr (length mvs0)))) *)
-    (*     with (Ptrofs.unsigned ofs0 + length mvs0). *)
-    (*   2:{ des. unfold Ptrofs.add. rewrite (Ptrofs.unsigned_repr (length _)). *)
-    (*       2:{ destruct ofs0; ss. nia. } *)
-    (*       rewrite Ptrofs.unsigned_repr. *)
-    (*       2:{ destruct ofs0; ss. nia. } et. } *)
-    (*   replace ((_points_to (blk m) (Ptrofs.unsigned ofs0) mvs0 q) *)
-    (*             ⋅ (_points_to (blk m) (Ptrofs.unsigned ofs0 + (length mvs0))) mvs1 q) *)
-    (*       with (_points_to (blk m) (Ptrofs.unsigned ofs0) (mvs0 ++ mvs1) q). *)
-    (*   2:{ unfold _points_to. unfold Auth.white. ur. ur. *)
-    (*       f_equal. ss. apply func_ext. i. ur. apply func_ext. i. ur. *)
-    (*       unfold __points_to. *)
-    (*       destruct dec; ss; *)
-    (*       destruct Coqlib.zle; ss; *)
-    (*       destruct Coqlib.zlt; ss; *)
-    (*       try destruct Coqlib.zle; ss; *)
-    (*       try destruct Coqlib.zlt; ss; *)
-    (*       try destruct Coqlib.zlt; ss; *)
-    (*       des_ifs; try rewrite app_length in *; try nia; *)
-    (*       try solve [rewrite nth_error_app1 in *; try nia; clarify *)
-    (*                 |rewrite nth_error_app2 in *; try nia; *)
-    (*                  replace (Z.to_nat _) with *)
-    (*                   ((Z.to_nat (x0 - Ptrofs.unsigned ofs0)) - length mvs0)%nat in Heq3 by nia; *)
-    (*                     clarify]. } *)
-    (*   iSplitL "A'"; ss. iExists _. iFrame. *)
-    (*   iPureIntro. des. *)
-    (*   unfold Vptrofs in *. des_ifs. *)
-    (*   unfold Ptrofs.add, Ptrofs.to_int64, Int64.add in *.  *)
-    (*   rewrite (Ptrofs.unsigned_repr (length mvs0)) in *. *)
-    (*   2,3: destruct ofs0; ss; nia. *)
-    (*   rewrite Ptrofs.unsigned_repr in *. *)
-    (*   2,3: destruct ofs0; ss; nia. *)
-    (*   rewrite app_length in *. nia. *)
-    admit "".
+    iIntros "[A B]". unfold points_to.
+    destruct (blk m); try solve [iDestruct "A" as "%"; clarify].
+    iDestruct "A" as "[? A]". iDestruct "B" as "[? B]". iFrame.
+    des_ifs; iDestruct "A" as (ofs) "[[[C A] %] %]"; des; clarify.
+    - unfold _has_offset. des_ifs. iDestruct "A" as "[? %]"; clarify.
+    - iDestruct "B" as (ofs0) "[[[D B] %] %]"; des; clarify.
+      rewrite <- Heq.
+      iPoseProof (_offset_dup with "A") as "[? A]".
+      iPoseProof (_has_offset_slide with "A") as "A".
+      iCombine "A B" as "A".
+      iPoseProof (_has_offset_unique with "A") as "%".
+      iClear "A". rewrite <- H9.
+      assert (X: Ptrofs.unsigned ofs + length mvs0 = Ptrofs.unsigned (Ptrofs.add ofs (Ptrofs.repr (length mvs0)))).
+      { unfold Ptrofs.add. destruct ofs. ss.
+        rewrite (Ptrofs.unsigned_repr (length _)); try nia.
+        rewrite (Ptrofs.unsigned_repr); et. nia. }
+      iCombine "C D" as "?". rewrite <- X. rewrite <- _points_to_content.
+      iExists _. iFrame. iPureIntro. rewrite app_length.
+      rewrite <- H9 in *. rewrite <- X in *.
+      splits; try nia.
+      unfold Val.addl, Vptrofs in *. des_ifs.
+      assert (X0: Int64.unsigned i + length mvs0 = Int64.unsigned (Int64.add i (Ptrofs.to_int64 (Ptrofs.repr (length mvs0))))).
+      { unfold Int64.add, Ptrofs.to_int64. destruct i. ss.
+        rewrite (Ptrofs.unsigned_repr (length _)); try nia.
+        change Ptrofs.max_unsigned with Int64.max_unsigned in *.
+        rewrite (Int64.unsigned_repr (length _)); try nia.
+        rewrite (Int64.unsigned_repr); et. nia. }
+      rewrite <- X0 in *. nia.
+    - iDestruct "B" as (ofs0) "[[[D B] %] %]"; des; clarify.
+      rewrite <- Heq.
+      iPoseProof (_offset_dup with "A") as "[? A]".
+      iPoseProof (_has_offset_slide with "A") as "A".
+      iCombine "A B" as "A".
+      iPoseProof (_has_offset_unique with "A") as "%".
+      iClear "A". rewrite <- H7.
+      assert (X: Ptrofs.unsigned ofs + length mvs0 = Ptrofs.unsigned (Ptrofs.add ofs (Ptrofs.repr (length mvs0)))).
+      { unfold Ptrofs.add. destruct ofs. ss.
+        rewrite (Ptrofs.unsigned_repr (length _)); try nia.
+        rewrite (Ptrofs.unsigned_repr); et. nia. }
+      iCombine "C D" as "?". rewrite <- X. rewrite <- _points_to_content.
+      iExists _. iFrame. iPureIntro. rewrite app_length.
+      rewrite <- H7 in *. rewrite <- X in *.
+      splits; try nia.
   Qed.
 
-  (* Lemma _capture_offset_comm *)
-  (*     vaddr i m ofs *)
-  (*   :  *)
-  (*     vaddr (≃_m) i ⊢ vaddr ⊨m# ofs ∗-∗ Vptrofs i ⊨m# ofs. *)
-  (* Proof. *)
-  (*   iIntros "A". *)
-  (*   iSplit; iIntros "B"; unfold _has_offset; des_ifs. *)
-  (*   - iDestruct "B" as "[B C]". iFrame. *)
-  (*     unfold captured_to. des_ifs. *)
-  (*     iDestruct "A" as "%". clarify. *)
-  (*     iDestruct "C" as "[A B]". *)
-  (*     iFrame.  *)
-  (*     iDestruct "B" as (a) "[A %]". *)
-  (*     iExists _. iFrame. iPureIntro. des. clarify. split; et. *)
-  (*     unfold Vptrofs in *. des_ifs. rewrite Ptrofs.of_int64_to_int64; et. *)
-  (*   - iDestruct "B" as "[B %]". iFrame. *)
-  (*     des. clarify. *)
-  (*     unfold Vptrofs in *. des_ifs. rewrite Ptrofs.of_int64_to_int64; et. *)
-  (*   - iDestruct "B" as "[B C]". iFrame. *)
-  (*     unfold captured_to. des_ifs. *)
-  (*     iDestruct "A" as "%". clarify. *)
-  (*     iDestruct "C" as "[A B]". *)
-  (*     iFrame.  *)
-  (*     iDestruct "B" as (a) "[A %]". *)
-  (*     iExists _. iFrame. iPureIntro. des. clarify. split; et. *)
-  (*     unfold Vptrofs in *. des_ifs. rewrite Ptrofs.of_int64_to_int64; et. *)
-  (*   - iDestruct "B" as "[B C]". iFrame. *)
-  (*     unfold captured_to. *)
-  (*     iDestruct "A" as "[A A']". *)
-  (*     iDestruct "C" as "[C B]". *)
-  (*     iDestruct "B" as (a) "[B %]". *)
-  (*     iDestruct "A'" as (a0) "[A' %]". *)
-  (*     des. clarify. *)
-  (*     iCombine "A' B" as "A'". *)
-  (*     iOwnWf "A'" as wfc. *)
-  (*     ur in wfc. specialize (wfc (blk m)). ur in wfc. *)
-  (*     unfold _has_base in *. des_ifs. *)
-  (*     iPureIntro. des. clarify. split; et. *)
-  (*     unfold Vptrofs in *. des_ifs. rewrite Ptrofs.of_int64_to_int64; et. *)
-  (* Qed. *)
+  Lemma equiv_refl_point m p q mvs
+    : p (↦_m,q) mvs  ⊢  p (↦_m,q) mvs ** p (≃_m) p.
+  Proof.
+    iIntros "A". unfold points_to.
+    destruct (blk m); try solve [iDestruct "A" as "%"; clarify].
+    iDestruct "A" as "[? A]".
+    des_ifs; iDestruct "A" as (ofs) "[[[C A] %] %]"; des; clarify.
+    - unfold _has_offset. des_ifs. iDestruct "A" as "[? %]"; clarify.
+    - iFrame. iPoseProof (_offset_dup with "A") as "[? A]".
+      iPoseProof (_offset_dup with "A") as "A".
+      iSplitR "A".
+      + iExists _. iFrame. iPureIntro. nia.
+      + iExists _. et.
+    - iFrame. iPoseProof (_offset_dup with "A") as "[? A]".
+      iPoseProof (_offset_dup with "A") as "A".
+      iSplitR "A".
+      + iExists _. iFrame. iPureIntro. nia.
+      + iExists _. et.
+  Qed.
 
-  (* Lemma capture_offset_comm *)
-  (*     vaddr i m tg q ofs *)
-  (*   :  *)
-  (*     vaddr (≃_m) i ⊢ vaddr (⊨_m,tg,q) ofs ∗-∗ Vptrofs i (⊨_m,tg,q) ofs. *)
-  (* Proof. *)
-  (*   iIntros "A". *)
-  (*   iPoseProof (_capture_offset_comm with "A") as "A". *)
-  (*   iSplit. *)
-  (*   - iIntros "[B C]". iPoseProof ("A" with "C") as "?". iFrame. *)
-  (*   - iIntros "[B C]". iPoseProof ("A" with "C") as "?". iFrame. *)
-  (* Qed. *)
+  Lemma equiv_refl_offset m p tg q ofs
+    : p (⊨_m,tg,q) ofs  ⊢  p (⊨_m,tg,q) ofs ** p (≃_m) p.
+  Proof.
+    iIntros "A". unfold has_offset.
+    destruct (blk m); try solve [iDestruct "A" as "%"; clarify].
+    iDestruct "A" as "[? A]".
+    iPoseProof (_offset_dup with "A") as "[? A]".
+    iPoseProof (_offset_dup with "A") as "A".
+    iSplitR "A"; iFrame. iExists _. et.
+  Qed.
 
+  Lemma equiv_sym p q m
+    : p (≃_m) q ⊢ q (≃_m) p.
+  Proof.
+    iIntros "A". unfold equiv_prov.
+    iDestruct "A" as (ofs) "[A B]".
+    iExists ofs. iFrame.
+  Qed.
 
-  (* Lemma capture_pointto_comm *)
-  (*     vaddr i m q mvs *)
-  (*   :  *)
-  (*     vaddr (≃_m) i ⊢ vaddr (↦_m,q) mvs ∗-∗ Vptrofs i (↦_m,q) mvs. *)
-  (* Proof. *)
-  (*   iIntros "A". *)
-  (*   iSplit; iIntros "B"; unfold points_to; des_ifs.  *)
-  (*   - iDestruct "B" as "[B C]". iFrame. *)
-  (*     iDestruct "C" as (ofs) "[[C D] %]". *)
-  (*     unfold Vptrofs in *. ss. des_ifs. *)
-  (*     iDestruct "A" as "%". *)
-  (*     des. clarify. iExists _. iSplitR "". *)
-  (*     { iSplitL "C"; ss. *)
-  (*       rewrite Ptrofs.to_int64_of_int64; et. } *)
-  (*     iPureIntro. rewrite Ptrofs.to_int64_of_int64; et. *)
-  (*   - iDestruct "B" as "[B C]". iFrame. *)
-  (*     iDestruct "C" as (ofs) "[[[C D] %] %]". *)
-  (*     unfold Vptrofs in *. des_ifs. *)
-  (*     iExists _. iSplit. *)
-  (*     { iPoseProof (_capture_offset_comm with "A") as "A". *)
-  (*       iPoseProof ("A" with "D") as "D". iFrame. ss. } *)
-  (*     unfold captured_to. *)
-  (*     iDestruct "A" as "[A B]". *)
-  (*     iDestruct "B" as (a) "[B %]". *)
-  (*     des. clarify. *)
-  (*     unfold _has_offset. *)
-  (*     iDestruct "D" as "[D %]". *)
-  (*     des. clarify. *)
-  (*     iPureIntro. split; et. *)
-  (*     replace (Int64.unsigned (Ptrofs.to_int64 i)) with (Ptrofs.unsigned i). *)
-  (*     2:{ unfold Ptrofs.to_int64. rewrite Int64.unsigned_repr; et. *)
-  (*         change Int64.max_unsigned with Ptrofs.max_unsigned. *)
-  (*         apply Ptrofs.unsigned_range_2. } *)
-  (*     assert (Ptrofs.unsigned (Ptrofs.sub i a) + Ptrofs.unsigned a + length mvs ≤ Ptrofs.max_unsigned) by nia. *)
-  (*     assert (Ptrofs.unsigned i ≤ Ptrofs.unsigned (Ptrofs.sub i a) + Ptrofs.unsigned a); try nia. *)
-  (*     unfold Ptrofs.sub. *)
-  (*     destruct (classic (0 ≤ Ptrofs.unsigned i - Ptrofs.unsigned a ≤ Ptrofs.max_unsigned)). *)
-  (*     { rewrite Ptrofs.unsigned_repr; nia. } *)
-  (*     pose proof (Ptrofs.unsigned_range_2 i). *)
-  (*     pose proof (Ptrofs.unsigned_range_2 a). *)
-  (*     assert (Ptrofs.unsigned i ≤ Ptrofs.unsigned a) by nia. *)
-  (*     pose proof (Ptrofs.unsigned_range_2 (Ptrofs.repr (Ptrofs.unsigned i - Ptrofs.unsigned a))). *)
-  (*     nia. *)
-  (*   - iDestruct "B" as "[B C]". iFrame. *)
-  (*     iDestruct "C" as (ofs) "[[C D] %]". *)
-  (*     unfold Vptrofs in *. ss. des_ifs. *)
-  (*     iDestruct "A" as "%". *)
-  (*     des. clarify. iExists _. iSplitR "". *)
-  (*     { iSplitL "C"; ss. *)
-  (*       rewrite Ptrofs.to_int64_of_int64; et. } *)
-  (*     iPureIntro. rewrite Ptrofs.to_int64_of_int64 in H5; et. *)
-  (*   - iDestruct "B" as "[B C]". iFrame. *)
-  (*     iDestruct "C" as (ofs) "[[[C D] %] %]". *)
-  (*     unfold Vptrofs in *. des_ifs. *)
-  (*     iExists _. iSplit. *)
-  (*     { iPoseProof (_capture_offset_comm with "A") as "A". *)
-  (*       iPoseProof ("A" with "D") as "D". iFrame. ss. } *)
-  (*     unfold captured_to. *)
-  (*     iDestruct "A" as "[A B]". *)
-  (*     iDestruct "B" as (a) "[B %]". *)
-  (*     des. clarify. *)
-  (* Qed. *)
+  Lemma equiv_trans p q r m
+    : p (≃_m) q ** q (≃_m) r 
+    ⊢ p (≃_m) r.
+  Proof.
+    iIntros "A". unfold equiv_prov.
+    iDestruct "A" as "[A B]".
+    iDestruct "A" as (ofs1) "[A A']". iDestruct "B" as (ofs2) "[B B']".
+    iCombine "A' B" as "A'". iPoseProof (_has_offset_unique with "A'") as "%". subst.
+    iExists ofs2. iFrame.
+  Qed.
+
+  Lemma equiv_dup p q m
+    : p (≃_m) q
+    ⊢ p (≃_m) q ** p (≃_m) q.
+  Proof.
+    unfold equiv_prov.
+    iIntros "A".
+    iDestruct "A" as (ofs) "[A B]".
+    iPoseProof (_offset_dup with "A") as "[A ?]".
+    iPoseProof (_offset_dup with "B") as "[B ?]".
+    iSplitL "A B"; iExists _; iFrame.
+  Qed.
+
+  Lemma capture_unique
+      p m i j
+    :
+      p (≃_m) (Vptrofs i) ** p (≃_m) (Vptrofs j) ⊢ ⌜i = j⌝.
+  Proof.
+    iIntros "[A B]".
+    iDestruct "A" as (ofs0) "[A' A]".
+    iDestruct "B" as (ofs1) "[B' B]".
+    iCombine "A' B'" as "C".
+    iPoseProof (_has_offset_unique with "C") as "%". clarify. iClear "C".
+    unfold _has_offset. des_ifs.
+    iDestruct "A" as "[_ A]".
+    iDestruct "B" as "[_ B]".
+    iDestruct "A" as (a0) "[A %]".
+    iDestruct "B" as (a1) "[B %]".
+    iCombine "A B" as "C".
+    iPoseProof (_has_base_unique with "C") as "%". clarify.
+    iPureIntro.
+    assert (i0 = i1).
+    { des. rewrite H4 in H3. clear - H3.
+      assert (Ptrofs.eq (Ptrofs.sub (Ptrofs.of_int64 i0) a1) (Ptrofs.sub (Ptrofs.of_int64 i1) a1) = true).
+      { rewrite H3. apply Ptrofs.eq_true. }
+      do 2 rewrite Ptrofs.sub_add_opp in H.
+      rewrite Ptrofs.translate_eq in H.
+      apply Ptrofs.same_if_eq in H.
+      apply (f_equal Ptrofs.to_int64) in H.
+      rewrite Ptrofs.to_int64_of_int64 in H; et.
+      rewrite Ptrofs.to_int64_of_int64 in H; et. }
+    subst. rewrite <- Heq in Heq1.
+    clear -Heq1. unfold Vptrofs in *. des_ifs.
+    replace intrange with intrange0 in * by apply proof_irrel.
+    rewrite <- Heq1 in Heq0. 
+    apply (f_equal Ptrofs.of_int64) in Heq0.
+    rewrite Ptrofs.of_int64_to_int64 in Heq0; et.
+    rewrite Ptrofs.of_int64_to_int64 in Heq0; et.
+  Qed.
+
+  (* TODO: have to impove lemma
+  Lemma alive_door p m tg f:
+      p (⊨_m,tg,f) Ptrofs.zero
+      ⊢ p (⊨_m,tg,f) Ptrofs.zero ** (∀q m' tg' f', (q (⊨_m',tg',f') Ptrofs.zero ** ptr_equiv p q) -* ⌜p = q⌝).
+  Proof.
+  Admitted. *)
 
   Lemma pointto_offset_notnull 
       vaddr m tg q ofs mvs
@@ -898,7 +637,7 @@ Section RULES.
   Proof.
   Admitted.
 
-  Lemma valid_ofs_same_meta
+  (* Lemma valid_ofs_same_meta
       vaddr m m' tg tg' q q' ofs ofs'
     : 
       vaddr (⊨_m,tg,q) ofs ** vaddr (⊨_m',tg',q') ofs' ** ⌜valid m ofs /\ valid m' ofs'⌝
@@ -906,62 +645,62 @@ Section RULES.
   Proof.
   Admitted.
 
-  (* Lemma same_addr_point_comm *)
-  (*     vaddr vaddr' m m' q i mvs *)
-  (*   :  *)
-  (*     vaddr (≃_m) i ** vaddr' (≃_m) i ** vaddr (↦_m', q) mvs *)
-  (*      ⊢ vaddr (↦_m', q) mvs. *)
-  (* Proof. *)
-  (* Admitted. *)
+  Lemma same_addr_point_comm
+      vaddr vaddr' m m' q i mvs
+    :
+      vaddr (≃_m) i ** vaddr' (≃_m) i ** vaddr (↦_m', q) mvs
+       ⊢ vaddr (↦_m', q) mvs.
+  Proof.
+  Admitted.
 
-  (* Lemma replace_meta_to_alive_point *)
-  (*     vaddr m0 m1 q mvs i *)
-  (*   : *)
-  (*     vaddr (↦_m0,q) mvs ** vaddr (≃_m1) i ⊢ vaddr (↦_m0,q) mvs ** vaddr (≃_m0) i. *)
-  (* Proof. *)
-  (*   iIntros "[A B]". *)
-  (*   unfold points_to, captured_to. *)
-  (*   des_ifs. *)
-  (*   - iFrame. *)
-  (*   - iDestruct "A" as "[A A']". *)
-  (*     iDestruct "B" as "[B B']". *)
-  (*     iDestruct "A'" as (ofs) "[[[C C'] %] %]". *)
-  (*     unfold _has_offset.  *)
-  (*     iDestruct "C'" as "[C' %]". *)
-  (*     des. clarify. *)
-  (*     iDestruct "B'" as (a) "[B' %]". *)
-  (*     des. clarify. rewrite H5. *)
-  (*     iAssert ⌜m0 = m1⌝ as "%". *)
-  (*     { iCombine "A B" as "D". iOwnWf "D" as wfc. *)
-  (*       iPureIntro. *)
-  (*       ur in wfc. specialize (wfc (blk m1)). *)
-  (*       ur in wfc. unfold _has_size in wfc. *)
-  (*       des_ifs. destruct m0. destruct m1. ss. clarify.  *)
-  (* Admitted. *)
+  Lemma replace_meta_to_alive_point
+      vaddr m0 m1 q mvs i
+    :
+      vaddr (↦_m0,q) mvs ** vaddr (≃_m1) i ⊢ vaddr (↦_m0,q) mvs ** vaddr (≃_m0) i.
+  Proof.
+    iIntros "[A B]".
+    unfold points_to, captured_to.
+    des_ifs.
+    - iFrame.
+    - iDestruct "A" as "[A A']".
+      iDestruct "B" as "[B B']".
+      iDestruct "A'" as (ofs) "[[[C C'] %] %]".
+      unfold _has_offset.
+      iDestruct "C'" as "[C' %]".
+      des. clarify.
+      iDestruct "B'" as (a) "[B' %]".
+      des. clarify. rewrite H5.
+      iAssert ⌜m0 = m1⌝ as "%".
+      { iCombine "A B" as "D". iOwnWf "D" as wfc.
+        iPureIntro.
+        ur in wfc. specialize (wfc (blk m1)).
+        ur in wfc. unfold _has_size in wfc.
+        des_ifs. destruct m0. destruct m1. ss. clarify.
+  Admitted.
 
-  (* Lemma replace_meta_to_alive_offset *)
-  (*     vaddr m0 m1 q tg ofs i *)
-  (*   : *)
-  (*     vaddr (⊨_m0,tg,q) ofs ** vaddr (≃_m1) i ⊢ vaddr (⊨_m0,tg,q) ofs ** vaddr (≃_m0) i. *)
-  (* Proof. *)
-  (*   iIntros "[A B]". *)
-  (*   unfold has_offset, captured_to. *)
-  (*   des_ifs. *)
-  (*   - iFrame. *)
-  (*   - iDestruct "A" as "[A A']". *)
-  (*     iDestruct "B" as "[B B']". *)
-  (*     unfold _has_offset. *)
-  (*     iDestruct "A'" as "[A' %]". *)
-  (*     des. clarify. *)
-  (*     iDestruct "B'" as (a) "[B' %]". *)
-  (*     des. clarify. rewrite H3. *)
-  (*     iAssert ⌜m0 = m1⌝ as "%". *)
-  (*     { iCombine "A' B" as "D". iOwnWf "D" as wfc. *)
-  (*       iPureIntro. *)
-  (*       ur in wfc. specialize (wfc (blk m1)). *)
-  (*       ur in wfc. unfold _has_size in wfc. *)
-  (*       des_ifs. destruct m0. destruct m1. ss. clarify.  *)
-  (* Admitted. *)
+  Lemma replace_meta_to_alive_offset
+      vaddr m0 m1 q tg ofs i
+    :
+      vaddr (⊨_m0,tg,q) ofs ** vaddr (≃_m1) i ⊢ vaddr (⊨_m0,tg,q) ofs ** vaddr (≃_m0) i.
+  Proof.
+    iIntros "[A B]".
+    unfold has_offset, captured_to.
+    des_ifs.
+    - iFrame.
+    - iDestruct "A" as "[A A']".
+      iDestruct "B" as "[B B']".
+      unfold _has_offset.
+      iDestruct "A'" as "[A' %]".
+      des. clarify.
+      iDestruct "B'" as (a) "[B' %]".
+      des. clarify. rewrite H3.
+      iAssert ⌜m0 = m1⌝ as "%".
+      { iCombine "A' B" as "D". iOwnWf "D" as wfc.
+        iPureIntro.
+        ur in wfc. specialize (wfc (blk m1)).
+        ur in wfc. unfold _has_size in wfc.
+        des_ifs. destruct m0. destruct m1. ss. clarify.
+  Admitted. *)
 
   Lemma _offset_ptr {eff} {K:eventE -< eff} v m ofs
     : 
@@ -977,8 +716,8 @@ Section RULES.
       v (⊨_m,tg,q) ofs ⊢ ⌜@cast_to_ptr eff K v = Ret v⌝.
   Proof.
     iIntros "A". unfold has_offset. des_ifs.
-    unfold _has_offset. des_ifs; ss.
-    all: admit "".
+    unfold _has_offset.
+    des_ifs; iDestruct "A" as "[_ [_ %]]"; clarify.
   Qed.
 
   Lemma points_to_is_ptr v m q mvs
@@ -1002,7 +741,7 @@ Section RULES.
     iIntros "A". unfold has_offset, _has_offset.
     destruct v; try solve [iDestruct "A" as "[A [A' %]]"; clarify];
       des_ifs; rewrite H3; et.
-    all: admit "contradiction".
+    all: iDestruct "A" as "[_ [_ %]]"; clarify.
   Qed.
 
   Lemma add_null_r v m tg q ofs: 
